Alternative recursor on Unicode.Utf8.WellFounded

Unicode/Basic.lean
@@ -545,7 +545,7 @@ where
 
 end Unicode
 
-/-
+/-!
 ## 1 byte
 0xxxxxxx ← a(0xxxxxxx)
 a
@@ -587,3 +587,120 @@ zzzzyyyy yyxxxxxx ← a(1110zzzz) b(10yyyyyy) c(10xxxxxx)
 - [UTF-8 processing using SIMD (SSE4)](https://woboq.com/blog/utf-8-processing-using-simd.html)
 - [Validating UTF-8 In Less Than One Instruction Per Byte](https://arxiv.org/pdf/2010.03090)
 -/
+
+#check Nat.rec
+#check Unicode.Utf8.Seq.WellFormed.rec
+def Unicode.Utf8.moreRec.{u} {σ} [seq : Seq σ] {motive : ∀ s, seq.good s → Sort u}
+    (s : Utf8 σ) (h₁ : seq.good s)
+    (one : seq.value s h₁ < 0x80 → seq.WellFormed (seq.next s h₁) → motive s h₁)
+    (two : ∀ h₂, InRange (seq.value s h₁) 0xC2 0xE0 → IsTrailing (seq.value (seq.next s h₁) h₂) →
+      seq.WellFormed (seq.next (seq.next s h₁) h₂) → motive s h₁)
+    (three : ∀ h₂ h₃, InRange (seq.value s h₁) 0xE0 0xF0 →
+      seq.WellFormed (seq.next (seq.next (seq.next s h₁) h₂) h₃) → motive s h₁)
+    (four : ∀ h₂ h₃ h₄, InRange (seq.value s h₁) 0xF0 0xF5 →
+      seq.WellFormed (seq.next (seq.next (seq.next (seq.next s h₁) h₂) h₃) h₄) → motive s h₁)
+  : motive s h₁ :=
+  let wf := s.2; let s := s.1
+  let A := seq.more s h₁; let s := A.2; let a := A.1
+  if ha' : a < 0x80 then
+    suffices _ from one ha' this
+    match wf with
+    | .zero hn => absurd h₁ hn
+    | .one _ h => h
+    | .two ha .. | .three₂ ha .. | .three₄ ha .. | .four₂ ha .. => absurd_le ha' ha.1
+    | .three₁ ha .. | .three₃ ha .. | .four₁ ha .. | .four₃ ha .. => absurd_eq ha' ha
+  else
+  have h₂ : seq.good s :=
+    match wf with
+    | .zero hn => absurd h₁ hn
+    | .one ha .. => absurd ha.2 ‹_›
+    | .more _ (.more h₂ _) => h₂
+  let B := seq.more s h₂; let s := B.2; let b := B.1
+  if ha' : a < 0xE0 then
+    suffices _ ∧ _ ∧ _ from two h₂ this.1 this.2.1 this.2.2
+    match wf with
+    | .zero hn => absurd h₁ hn
+    | .one ha .. => absurd ha.2 ‹_›
+    | .two ha hb h => ⟨ha, hb, h⟩
+    | .three₂ ha .. | .three₄ ha .. | .four₂ ha .. => absurd_le ha' ha.1
+    | .three₁ ha .. | .three₃ ha .. | .four₁ ha .. | .four₃ ha .. => absurd_eq ha' ha
+  else
+  have h₃ : seq.good s :=
+    match wf with
+    | .zero hn => absurd h₁ hn
+    | .one ha .. | .two ha .. => absurd ha.2 ‹_›
+    | .more _ (.more _ (.more h₃ _)) => h₃
+  let C := seq.more s h₃; let s := C.2; let c := C.1
+  have ha'' : 0xE0 ≤ a := Nat.le_of_not_lt ha'
+  if ha' : a < 0xF0 then
+    suffices _ ∧ _ from three h₂ h₃ this.1 this.2
+    match wf with
+    | .zero hn => absurd h₁ hn
+    | .one ha .. | .two ha .. => absurd ha.2 ‹_›
+    | .three₂ ha _ _ h | .three₄ ha _ _ h => ⟨⟨ha'', Nat.lt_of_lt_of_le ha.2 (by decide)⟩, h⟩
+    | .three₁ ha _ _ h | .three₃ ha _ _ h => ⟨⟨ha'', ha ▸ by decide⟩, h⟩
+    | .four₂ ha .. => absurd_le ha' ha.1
+    | .four₁ ha .. | .four₃ ha .. => absurd_eq ha' ha
+  else
+  have ha' : a ≥ 0xF0 := Nat.le_of_not_lt ha'
+  have h₄ : seq.good s :=
+    match wf with
+    | .zero hn => absurd h₁ hn
+    | .one ha .. | .two ha .. | .three₂ ha .. | .three₄ ha .. => absurd_le ha.2 ha'
+    | .three₁ ha .. | .three₃ ha .. => absurd_eq' ha ha'
+    | .more _ (.more _ (.more _ (.more h₄ _))) => h₄
+  let D := seq.more s h₄; let s := D.2; let d := D.1
+    suffices _ ∧ _ from four h₂ h₃ h₄ this.1 this.2
+    match wf with
+    | .zero hn => absurd h₁ hn
+    | .one ha .. | .two ha .. | .three₂ ha .. | .three₄ ha .. => absurd_le ha.2 ha'
+    | .three₁ ha .. | .three₃ ha .. => absurd_eq' ha ha'
+    | .four₂ ha _ _ _ h => ⟨⟨ha', Nat.lt_trans ha.2 Nat.le.refl⟩, h⟩
+    | .four₁ ha _ _ _ h | .four₃ ha _ _ _ h => ⟨⟨ha', ha ▸ by decide⟩, h⟩
+where
+  absurd_le {α} {x a b : Utf8.CodeUnit} (ha : x < a) (hb : b ≤ x) (h : a ≤ b := by decide) : α :=
+    nomatch Nat.lt_le_asymm ha (Nat.le_trans h hb)
+  absurd_eq {α} {x a b : Utf8.CodeUnit} (ha : x < a) (hb : x = b) (h : a ≤ b := by decide) : α :=
+    nomatch Nat.lt_le_asymm ha (hb ▸ h)
+  absurd_eq' {α} {x a b : Utf8.CodeUnit} (ha : x = a) (hb : b ≤ x) (h : a < b := by decide) : α :=
+    absurd_eq h ha.symm hb
+
+open Unicode in
+example {σ} [seq : Utf8.Seq σ] : Utf32.Seq (Utf8 σ) where
+  good s := seq.good s
+  more s (h₁ : seq.good s) := show Utf32.CodeUnit × Utf8 σ from
+    s.moreRec h₁ (motive := fun _ _ => Utf32.CodeUnit × Utf8 σ)
+      (fun _ h => show Utf32.CodeUnit × Utf8 σ from
+        let A := seq.more s h₁; let s := A.2; let a := A.1
+        -- 0xxxxxxx ← 0xxxxxxx
+        ⟨a.toUInt32, s, h⟩)
+      (fun h₂ _ _ h => show Utf32.CodeUnit × Utf8 σ from
+        let A := seq.more s h₁; let s := A.2; let a := A.1
+        let B := seq.more s h₂; let s := B.2; let b := B.1
+        -- 00000yyy yyxxxxxx ← 110yyyyy 10xxxxxx
+        let y := a.toBitVec.extractLsb' 0 5
+        let x := b.toBitVec.extractLsb' 0 6
+        ⟨toUInt32 (y ++ x), s, h⟩)
+      (fun h₂ h₃ _ h => show Utf32.CodeUnit × Utf8 σ from
+        let A := seq.more s h₁; let s := A.2; let a := A.1
+        let B := seq.more s h₂; let s := B.2; let b := B.1
+        let C := seq.more s h₃; let s := C.2; let c := C.1
+        -- zzzzyyyy yyxxxxxx ← 1110zzzz 10yyyyyy 10xxxxxx
+        let z := a.toBitVec.extractLsb' 0 4
+        let y := b.toBitVec.extractLsb' 0 6
+        let x := c.toBitVec.extractLsb' 0 6
+        ⟨toUInt32 (z ++ y ++ x), s, h⟩)
+      (fun h₂ h₃ h₄ _ h => show Utf32.CodeUnit × Utf8 σ from
+        let A := seq.more s h₁; let s := A.2; let a := A.1
+        let B := seq.more s h₂; let s := B.2; let b := B.1
+        let C := seq.more s h₃; let s := C.2; let c := C.1
+        let D := seq.more s h₄; let s := D.2; let d := D.1
+        -- 000uuuuu zzzzyyyy yyxxxxxx ← 11110uuu 10uuzzzz 10yyyyyy 10xxxxxx
+        let u := a.toBitVec.extractLsb' 0 3
+        let z := b.toBitVec.extractLsb' 0 4
+        let y := c.toBitVec.extractLsb' 0 6
+        let x := d.toBitVec.extractLsb' 0 6
+        ⟨toUInt32 (u ++ z ++ y ++ x), s, h⟩)
+where
+  toUInt32 {w} (x : BitVec w) (h : w ≤ 32 := by decide) : UInt32 :=
+    .mk (x.setWidth' h)
